Port correctness

RegexCorrectness/NFA/VM/Correctness.lean
@@ -2,7 +2,7 @@ import Regex.NFA.VM.Basic
 import RegexCorrectness.NFA.Transition
 import RegexCorrectness.NFA.Correctness
 
-theorem Array.isEmpty_iff {α} (a : Array α) : a.isEmpty ↔ a = #[] := by
+theorem Array.isEmpty_iff {α} {a : Array α} : a.isEmpty ↔ a = #[] := by
   have : a.isEmpty ↔ a.data = [] := by
     simp [Array.isEmpty, Array.size]
     match a.data with
@@ -23,6 +23,11 @@ theorem Array.mem_back' {a : Array α} (hemp : ¬ a.isEmpty) : a.back' hemp ∈ 
 theorem Array.mem_push (a : Array α) (x y : α) :
   y ∈ a.push x ↔ y ∈ a ∨ y = x := by
   unfold Array.push
+  simp [Array.mem_def]
+
+@[simp]
+theorem Array.mem_of_push (a : Array α) (x : α) :
+  x ∈ a.push x := by
   simp [Array.mem_def]
 
 theorem Array.push_pop_eq (a : Array α) (hemp : ¬ a.isEmpty) :
@@ -59,7 +64,7 @@ theorem Array.mem_of_mem_pop (a : Array α) (x : α) (mem : x ∈ a.pop) :
   x ∈ a := by
   cases decEq a.isEmpty true with
   | isTrue hemp =>
-    have := (Array.isEmpty_iff _).mp hemp
+    have := (Array.isEmpty_iff).mp hemp
     subst this
     simp at mem
   | isFalse hemp =>
@@ -102,7 +107,7 @@ theorem εClosureTR_spec {i : Fin nfa.nodes.size} {inBounds : nfa.inBounds} :
     unfold εClosureTR
     split
     case inl hemp =>
-      have : stack = #[] := (Array.isEmpty_iff _).mp hemp
+      have : stack = #[] := (Array.isEmpty_iff).mp hemp
       exact this ▸ inv₀
     case inr hemp =>
       set n := stack.back' hemp with hn
@@ -574,3 +579,451 @@ theorem NFA.match_iff_regex_matches {s : String} (eq : compile r = nfa) :
     exact match_eq_matchList ▸ this
 
 end NFA
+
+namespace NFAa.VM
+
+open NFA.VM
+
+theorem mem_εStep_iff_εClosure_sub {nfa : NFAa} {S : Set Nat} :
+  (∀ i ∈ S, (_ : i < nfa.nodes.size) → ∀ j ∈ nfa[i].εStep, j ∈ S) ↔
+  ∀ i ∈ S, nfa.εClosure i ⊆ S := by
+  apply Iff.intro
+  . intro assm i mem
+    intro k cls
+    induction cls with
+    | base => exact mem
+    | @step i j k step _ ih =>
+      cases Nat.decLt i nfa.nodes.size with
+      | isTrue lt =>
+        simp [εStep, lt] at step
+        exact ih (assm i mem lt j step)
+      | isFalse nlt => simp [εStep, nlt] at step
+  . intro assm i mem _ j step
+    apply Set.mem_of_mem_of_subset _ (assm i mem)
+    exact εClosure.step (εStep_of_εStep step) .base
+
+def εClosureTRa_spec.inv (nfa : NFAa) (i : Fin nfa.nodes.size)
+  (visited : NodeSet nfa.nodes.size) (stack : Array (Fin nfa.nodes.size)) : Prop :=
+  (visited.get i ∨ i ∈ stack) ∧
+  (∀ i j, visited.get i → j.val ∈ nfa[i].εStep → visited.get j ∨ j ∈ stack) ∧
+  (∀ j, (visited.get j ∨ j ∈ stack) → j.val ∈ nfa.εClosure i)
+
+theorem εClosureTRa_spec.case_visited (inv₀ : inv nfa i visited stack)
+  (hemp : ¬ stack.isEmpty) (hvis : NodeSet.get visited (Array.back' stack hemp)) :
+  inv nfa i visited stack.pop := by
+  simp [inv] at *
+  set n := Array.back' stack hemp
+  obtain ⟨h₁, h₂, h₃⟩ := inv₀
+  refine ⟨?_, ?_, ?_⟩
+  . cases h₁ with
+    | inl vis => exact .inl vis
+    | inr stk =>
+      cases decEq i n with
+      | isTrue eq => exact .inl (eq ▸ hvis)
+      | isFalse ne => exact .inr (Array.mem_pop _ _ _ stk ne)
+  . intro i j mem step
+    cases h₂ i j mem step with
+    | inl vis => exact .inl vis
+    | inr stk =>
+      -- TODO: Looks like a duplication
+      cases decEq j n with
+      | isTrue eq => exact .inl (eq ▸ hvis)
+      | isFalse ne => exact .inr (Array.mem_pop _ _ _ stk ne)
+  . intro j h
+    apply h₃
+    cases h with
+    | inl vis => exact .inl vis
+    | inr stk => exact .inr (Array.mem_of_mem_pop _ _ stk)
+
+theorem εClosureTRa_spec.case_epsilon (inv₀ : inv nfa i visited stack)
+  (hemp : ¬ stack.isEmpty) (hvis : ¬ NodeSet.get visited (Array.back' stack hemp))
+  (hn : nfa.nodes[(Array.back' stack hemp).val] = NFA.Node.epsilon next) :
+  inv nfa i (visited.set (Array.back' stack hemp)) (stack.pop.push ⟨next, isLt⟩) := by
+  simp [inv] at *
+  set n := Array.back' stack hemp
+  obtain ⟨h₁, h₂, h₃⟩ := inv₀
+  refine ⟨?_, ?_, ?_⟩
+  . cases h₁ with
+    | inl vis => simp [NodeSet.get_set, vis]
+    | inr stk =>
+      cases Array.mem_pop_or_eq_of_mem _ _ hemp stk with
+      | inl stk => exact Or.inr ((Array.mem_push _ _ _).mpr (.inl stk))
+      | inr eq => simp [eq]
+  . intro i j mem step
+    rw [NodeSet.get_set] at mem
+    split at mem
+    case inl eq =>
+      simp [←eq, NFA.Node.εStep, get_eq_nodes_get, hn] at step
+      simp [←step]
+    case inr ne =>
+      cases h₂ i j mem step with
+      | inl vis => simp [NodeSet.get_set, vis]
+      | inr stk =>
+          cases Array.mem_pop_or_eq_of_mem _ _ hemp stk with
+          | inl stk => exact Or.inr ((Array.mem_push _ _ _).mpr (.inl stk))
+          | inr eq => simp [eq]
+  . intro j mem
+    cases mem with
+    | inl vis =>
+      rw [NodeSet.get_set] at vis
+      split at vis
+      case inl eq =>
+        rw [←eq]
+        exact h₃ n (.inr (Array.mem_back' hemp))
+      case inr ne => exact h₃ j (.inl vis)
+    | inr stk =>
+      cases (Array.mem_push _ _ _).mp stk with
+      | inl stk => exact h₃ j (.inr (Array.mem_of_mem_pop _ _ stk))
+      | inr eq =>
+        simp [eq]
+        have cls : n.val ∈ nfa.εClosure i := h₃ n (.inr (Array.mem_back' hemp))
+        have step : next ∈ nfa.εStep n := by
+          simp [εStep, NFA.Node.εStep, get_eq_nodes_get, hn]
+        exact εClosure_snoc cls step
+
+theorem εClosureTRa_spec.case_split (inv₀ : inv nfa i visited stack)
+  (hemp : ¬ stack.isEmpty) (hvis : ¬ NodeSet.get visited (Array.back' stack hemp))
+  (hn : nfa.nodes[(Array.back' stack hemp).val] = NFA.Node.split next₁ next₂) :
+  inv nfa i (visited.set (Array.back' stack hemp)) ((stack.pop.push ⟨next₁, isLt₁⟩).push ⟨next₂, isLt₂⟩) := by
+  simp [inv] at *
+  set n := Array.back' stack hemp
+  obtain ⟨h₁, h₂, h₃⟩ := inv₀
+  refine ⟨?_, ?_, ?_⟩
+  . cases h₁ with
+    | inl vis => simp [NodeSet.get_set, vis]
+    | inr stk =>
+      cases Array.mem_pop_or_eq_of_mem _ _ hemp stk with
+      | inl stk =>
+        exact Or.inr ((Array.mem_push _ _ _).mpr (.inl ((Array.mem_push _ _ _).mpr (.inl stk))))
+      | inr eq => simp [eq]
+  . intro i j mem step
+    rw [NodeSet.get_set] at mem
+    split at mem
+    case inl eq =>
+      simp [NFA.Node.εStep, get_eq_nodes_get, ←eq, hn] at step
+      cases step with
+      | inl eq₁ => simp [←eq₁, Array.mem_push]
+      | inr eq₂ => simp [←eq₂]
+    case inr ne =>
+      cases h₂ i j mem step with
+      | inl vis => simp [NodeSet.get_set, vis]
+      | inr stk =>
+        cases Array.mem_pop_or_eq_of_mem _ _ hemp stk with
+        | inl stk =>
+          exact Or.inr ((Array.mem_push _ _ _).mpr (.inl ((Array.mem_push _ _ _).mpr (.inl stk))))
+        | inr eq => simp [eq]
+  . intro j mem
+    have ncls : n.val ∈ nfa.εClosure i := h₃ n (.inr (Array.mem_back' hemp))
+    cases mem with
+    | inl vis =>
+      rw [NodeSet.get_set] at vis
+      split at vis
+      case inl eq => exact eq ▸ ncls
+      case inr ne => exact h₃ j (.inl vis)
+    | inr stk =>
+      cases (Array.mem_push _ _ _).mp stk with
+      | inl stk =>
+        cases (Array.mem_push _ _ _).mp stk with
+        | inl stk => exact h₃ j (.inr (Array.mem_of_mem_pop _ _ stk))
+        | inr eq =>
+          simp [eq]
+          have step : next₁ ∈ nfa.εStep n := by
+            simp [εStep, NFA.Node.εStep, get_eq_nodes_get, hn]
+          exact εClosure_snoc ncls step
+      | inr eq =>
+        simp [eq]
+        have step : next₂ ∈ nfa.εStep n := by
+          simp [εStep, NFA.Node.εStep, get_eq_nodes_get, hn]
+        exact εClosure_snoc ncls step
+
+theorem εClosureTRa_spec.case_else (inv₀ : inv nfa i visited stack)
+  (hemp : ¬ stack.isEmpty) (hvis : ¬ NodeSet.get visited (Array.back' stack hemp))
+  (hn₁ : ∀ (next : Nat), ¬ nfa.nodes[(Array.back' stack hemp).val] = NFA.Node.epsilon next)
+  (hn₂ : ∀ (next₁ next₂ : Nat), ¬ nfa.nodes[(Array.back' stack hemp).val] = NFA.Node.split next₁ next₂) :
+  inv nfa i (visited.set (Array.back' stack hemp)) stack.pop := by
+  simp [inv] at *
+  set n := Array.back' stack hemp
+  obtain ⟨h₁, h₂, h₃⟩ := inv₀
+  refine ⟨?_, ?_, ?_⟩
+  . cases h₁ with
+    | inl vis => simp [NodeSet.get_set, vis]
+    | inr stk =>
+      cases Array.mem_pop_or_eq_of_mem _ _ hemp stk with
+      | inl stk => exact Or.inr stk
+      | inr eq => simp [eq]
+  . intro i j mem step
+    rw [NodeSet.get_set] at mem
+    split at mem
+    case inl eq =>
+      exfalso
+      simp [eq.symm, NFA.Node.εStep] at step
+      split at step
+      next next hn => exact absurd hn (hn₁ next)
+      next next₁ next₂ hn => exact absurd hn (hn₂ next₁ next₂)
+      next hn => contradiction
+    case inr ne =>
+      cases h₂ i j mem step with
+      | inl vis => simp [NodeSet.get_set, vis]
+      | inr stk =>
+        cases Array.mem_pop_or_eq_of_mem _ _ hemp stk with
+        | inl stk => exact Or.inr stk
+        | inr eq => simp [eq]
+  . intro j mem
+    cases mem with
+    | inl vis =>
+      cases decEq j n with
+      | isTrue eq =>
+        rw [eq]
+        have : n ∈ stack := Array.mem_back' hemp
+        exact h₃ n (.inr this)
+      | isFalse neq =>
+        rw [NodeSet.get_set_ne] at vis
+        . exact h₃ j (.inl vis)
+        . intro h
+          exact neq (Fin.eq_of_val_eq h).symm
+    | inr stk =>
+      have : j ∈ stack := Array.mem_of_mem_pop _ _ stk
+      exact h₃ j (.inr this)
+
+-- The case analysis takes a bit of time, so we split each branch as lemmas
+theorem εClosureTRa_spec.go (nfa : NFAa) (i : Fin nfa.nodes.size) {visited stack}
+  (inv₀ : inv nfa i visited stack) :
+  inv nfa i (εClosureTRa nfa visited stack) #[] := by
+  unfold εClosureTRa
+  split
+  case inl hemp => exact (Array.isEmpty_iff.mp hemp) ▸ inv₀
+  case inr hemp =>
+    have : stack.pop.size < stack.size := Array.lt_size_of_pop_of_not_empty _ hemp
+    simp
+    split
+    case inl hvis => exact go nfa i (case_visited inv₀ hemp hvis)
+    case inr hvis =>
+      have : (visited.set (Array.back' stack hemp)).count_unset < visited.count_unset :=
+        visited.lt_count_unset _ hvis
+      split
+      next hn => exact go nfa i (case_epsilon inv₀ hemp hvis hn)
+      next hn => exact go nfa i (case_split inv₀ hemp hvis hn)
+      next hn₁ hn₂ => exact go nfa i (case_else inv₀ hemp hvis hn₁ hn₂)
+termination_by _ => (visited.count_unset, stack.size)
+
+theorem εClosureTRa_spec {nfa : NFAa} {i : Fin nfa.nodes.size} :
+  ∀ j, (εClosureTRa nfa .empty #[i]).get j ↔ j.val ∈ nfa.εClosure i := by
+  have inv₀ : εClosureTRa_spec.inv nfa i .empty #[i] := by
+    simp [εClosureTRa_spec.inv]
+    exact .base
+  have ⟨h₁, h₂, h₃⟩ := εClosureTRa_spec.go nfa i inv₀
+  simp at h₁ h₂ h₃
+  intro j
+  apply Iff.intro
+  . exact h₃ j
+  . intro h
+    let S := { j | ∃ lt : j < nfa.nodes.size, (εClosureTRa nfa .empty #[i]).get ⟨j, lt⟩ }
+    have mem : i.val ∈ S := by
+      simp [h₁]
+    have : ∀ j ∈ S, (_ : j < nfa.nodes.size) → ∀ k ∈ nfa[j].εStep, k ∈ S := by
+      intro j mem _ k step
+      simp at mem
+      obtain ⟨_, get⟩ := mem
+      simp
+      have klt : k < nfa.nodes.size := lt_of_εStep step
+      have := h₂ _ ⟨k, klt⟩ get
+      refine ⟨klt, this ?_⟩
+      simp [step]
+
+    have := mem_εStep_iff_εClosure_sub.mp this i mem
+    have := Set.mem_of_mem_of_subset h this
+    simp at this
+    exact this
+
+def charStepTRa_spec.inv (nfa : NFAa) (c : Char) (init : NodeSet nfa.nodes.size)
+  (accum : NodeSet nfa.nodes.size) (i : Nat) : Prop :=
+  ∀ k, accum.get k ↔ k.val ∈ nfa.stepSet { j | j < i ∧ ∃ h : j < nfa.nodes.size, init.get ⟨j, h⟩ } c
+
+theorem charStepTRa_spec.lem (nfa : NFAa) (init : NodeSet nfa.nodes.size)
+  (i : Nat) (hlt : i < nfa.nodes.size) :
+  { j | j < i + 1 ∧ ∃ h : j < nfa.nodes.size, init.get ⟨j, h⟩ } =
+  if init.get ⟨i, hlt⟩ then
+    { j | j < i ∧ ∃ h : j < nfa.nodes.size, init.get ⟨j, h⟩ } ∪ {i}
+  else
+    { j | j < i ∧ ∃ h : j < nfa.nodes.size, init.get ⟨j, h⟩ } := by
+  split
+  case inl hset =>
+    apply Set.eq_of_subset_of_subset
+    . intro j
+      simp
+      intro lt₁ lt₂ hset'
+      cases Nat.lt_or_eq_of_le (Nat.le_of_lt_succ lt₁) with
+      | inl lt₃ => exact .inr ⟨lt₃, lt₂, hset'⟩
+      | inr eq => exact .inl eq
+    . intro j
+      simp
+      intro h
+      match h with
+      | .inl eq => simp [eq, hlt, hset]
+      | .inr ⟨lt₁, lt₂, hset'⟩ => exact ⟨Nat.lt_trans lt₁ (Nat.lt_succ_self _), lt₂, hset'⟩
+  case inr hset =>
+    apply Set.eq_of_subset_of_subset
+    . intro j
+      simp
+      intro lt₁ lt₂ hset'
+      cases Nat.lt_or_eq_of_le (Nat.le_of_lt_succ lt₁) with
+      | inl lt₃ => exact ⟨lt₃, lt₂, hset'⟩
+      | inr eq => simp [eq, hset] at hset'
+    . intro j
+      simp
+      intro lt₁ lt₂ hset'
+      exact ⟨Nat.lt_trans lt₁ (Nat.lt_succ_self _), lt₂, hset'⟩
+
+theorem charStepTRa_spec.go (nfa : NFAa) (c : Char) (init : NodeSet nfa.nodes.size)
+  (accum : NodeSet nfa.nodes.size) (i : Nat) (hle : i ≤ nfa.nodes.size)
+  (inv₀ : inv nfa c init accum i) :
+  ∀ k, ((charStepTRa.go nfa c init accum i hle)).get k ↔
+  k.val ∈ nfa.stepSet { j | ∃ h : j < nfa.nodes.size, init.get ⟨j, h⟩ } c := by
+  unfold charStepTRa.go
+  split
+  case inl eq =>
+    have : { j | j < i ∧ ∃ h : j < nfa.nodes.size, init.get ⟨j, h⟩ }
+      = { j | ∃ h : j < nfa.nodes.size, init.get ⟨j, h⟩ } := by
+      apply Set.eq_of_subset_of_subset
+      . intro j h
+        simp at *
+        obtain ⟨_, ⟨lt, mem⟩⟩ := h
+        exact ⟨lt, mem⟩
+      . intro j h
+        simp at *
+        exact ⟨eq ▸ h.1, h⟩
+    rw [inv, this] at inv₀
+    exact inv₀
+  case inr ne =>
+    simp
+    have hlt : i < nfa.nodes.size := Nat.lt_of_le_of_ne hle ne
+    apply go nfa c init _ (i + 1) hlt
+    split
+    case inl hset =>
+      simp [inv, lem nfa init i hlt, hset, stepSet_insert_distrib]
+      split
+      next next hn =>
+        split
+        case inl eqc =>
+          intro k
+          apply Iff.intro
+          . intro hset
+            simp [NodeSet.merge_get] at hset
+            cases hset with
+            | inl hset => exact .inl ((inv₀ k).mp hset)
+            | inr hset =>
+              apply Or.inr
+              simp [εClosureTRa_spec k] at hset
+              simp [stepSet, εClosureSet]
+              refine ⟨next, ?_, hset⟩
+              simp [charStep, get_eq_nodes_get, NFA.Node.charStep, hn, eqc, hlt]
+          . intro hset
+            simp [NodeSet.merge_get]
+            cases hset with
+            | inl hset => exact .inl ((inv₀ k).mpr hset)
+            | inr hset =>
+              apply Or.inr
+              simp [εClosureTRa_spec k]
+              simp [stepSet, εClosureSet, charStep, get_eq_nodes_get, NFA.Node.charStep, hn, eqc, hlt] at hset
+              exact hset
+        case inr nec =>
+          have : nfa.stepSet {i} c = ∅ := by
+            simp [stepSet, charStep, NFA.Node.charStep, get_eq_nodes_get, hn, nec]
+          simp [this]
+          exact inv₀
+      next hn =>
+        have : nfa.stepSet {i} c = ∅ := by
+          simp [stepSet, charStep, NFA.Node.charStep, get_eq_nodes_get, hn]
+        simp [this]
+        exact inv₀
+    case inr hset =>
+      simp [inv, lem nfa init i hlt, hset]
+      exact inv₀
+termination_by _ => nfa.nodes.size - i
+
+theorem charStepTRa_spec (nfa : NFAa) (c : Char) (init : NodeSet nfa.nodes.size) :
+  ∀ k, (charStepTRa nfa c init).get k ↔
+  k.val ∈ nfa.stepSet { j | ∃ h : j < nfa.nodes.size, init.get ⟨j, h⟩ } c := by
+  have inv₀ : charStepTRa_spec.inv nfa c init .empty 0 := by
+    simp [charStepTRa_spec.inv, Nat.not_lt_zero]
+  exact charStepTRa_spec.go nfa c init .empty 0 (Nat.zero_le _) inv₀
+
+def matchList (nfa : NFAa) (cs : List Char) : Bool :=
+  let ns := εClosureTRa nfa .empty #[nfa.start]
+  let ns := go nfa cs ns
+  -- This assumes that the first node is the accepting node
+  ns.get ⟨0, nfa.zero_lt_size⟩
+where
+  go (nfa : NFAa) (cs : List Char) (ns : NodeSet nfa.nodes.size) : NodeSet nfa.nodes.size :=
+    List.foldl (fun ns c => charStepTRa nfa c ns) ns cs
+
+theorem matchList.go_eq_foldl_stepSet {nfa : NFAa} {ns : NodeSet nfa.nodes.size} {cs : List Char} :
+  ∀ j, (go nfa cs ns).get j ↔
+    j.val ∈ List.foldl nfa.stepSet { i | ∃ h : i < nfa.nodes.size, ns.get ⟨i, h⟩ } cs := by
+  induction cs generalizing ns with
+  | nil => simp [go]
+  | cons c cs ih =>
+    simp [go]
+    unfold go at ih
+    have spec := charStepTRa_spec nfa c ns
+    intro j
+    rw [ih j]
+    congr!
+    simp [spec]
+    apply Set.eq_of_subset_of_subset
+    . intro i
+      simp
+    . intro i mem
+      simp [mem]
+      exact lt_of_mem_stepSet mem
+
+theorem evalFrom_iff_matchList {nfa : NFAa} {cs : List Char} :
+  0 ∈ nfa.evalFrom {nfa.start.val} cs ↔ matchList nfa cs := by
+  unfold NFAa.evalFrom matchList
+  simp [matchList.go_eq_foldl_stepSet, εClosureTRa_spec]
+  congr! 2
+  simp [εClosureSet]
+  apply Set.eq_of_subset_of_subset
+  . intro i mem
+    simp
+    exact ⟨lt_of_εClosure_right nfa.start.isLt mem, mem⟩
+  . intro i mem
+    simp at mem
+    exact mem.right
+
+theorem match.go_eq_matchList.go {nfa : NFAa} {ns : NodeSet nfa.nodes.size}
+  {it : String.Iterator} {cs cs' : List Char} (v : it.ValidFor cs cs') :
+  NFAa.match.go nfa it ns = matchList.go nfa cs' ns := by
+  induction cs' generalizing it cs ns with
+  | nil =>
+    unfold NFAa.match.go matchList.go
+    have : it.atEnd := v.atEnd.mpr rfl
+    simp [this]
+  | cons c cs' ih =>
+    unfold NFAa.match.go matchList.go
+    have : ¬ it.atEnd := by
+      intro h
+      have := v.atEnd.mp h
+      contradiction
+    simp [this]
+    have : it.curr = c := by
+      simp [v.curr]
+    simp [this]
+    exact ih v.next
+
+theorem match_eq_matchList {nfa : NFAa} {s : String} :
+  nfa.match s ↔ matchList nfa s.data := by
+  unfold NFAa.match matchList
+  simp
+  rw [match.go_eq_matchList.go s.validFor_mkIterator]
+
+theorem evalFrom_iff_match {nfa : NFAa} {s : String} :
+  nfa.match s ↔ 0 ∈ nfa.evalFrom {nfa.start.val} s.data := by
+  rw [match_eq_matchList, evalFrom_iff_matchList]
+
+theorem match_iff_regex_matches (eq : NFAa.compile r = nfa) :
+  nfa.match s ↔ r.matches s := by
+  rw [evalFrom_iff_match]
+  exact ⟨matches_of_compile_evalFrom eq, evalFrom_of_compile_matches eq⟩
+
+end NFAa.VM
